tests/micro-benchmarks/TestQueue.fst
@@ -8,17 +8,17 @@ let my_queue = enqueue 3 (enqueue 2 (enqueue 1 Q.empty))
 let my_seq = Seq.cons 1 (Seq.cons 2 (Seq.cons 3 Seq.empty))
 
 let _ = assert 
-  (Q.eq my_queue (queue_of_seq my_seq))
+  (Q.equal my_queue (queue_of_seq my_seq))
 let _ = assert 
-  (Q.eq (enqueue 4 my_queue) 
+  (Q.equal (enqueue 4 my_queue) 
         (queue_of_seq (Seq.snoc my_seq 4)))
 let _ = assert 
   (fst (dequeue my_queue) == 1)
 let _ = assert 
-  (Q.eq (snd (dequeue my_queue)) 
+  (Q.equal (snd (dequeue my_queue)) 
         (enqueue 3 (enqueue 2 Q.empty)))
 let _ = assert 
-  (Q.eq (snd (dequeue (enqueue 1 Q.empty))) 
+  (Q.equal (snd (dequeue (enqueue 1 Q.empty))) 
         Q.empty)
 let _ = assert 
   (peek my_queue == 1)
